\documentclass{report}
\usepackage[utf8]{inputenc}
\usepackage{upgreek}
\usepackage{amsmath}
\def\undertilde#1{\mathord{\vtop{\ialign{##\crcr
$\hfil\displaystyle{#1}\hfil$\crcr\noalign{\kern1.5pt\nointerlineskip}
$\hfil\tilde{}\hfil$\crcr\noalign{\kern1.5pt}}}}}
\def\therefore{\boldsymbol{\text{ }
\leavevmode
\lower0.4ex\hbox{$\cdot$}
\kern-.4em\raise0.5ex\hbox{$\cdot$}
\kern-0.55em\lower0.4ex\hbox{$\cdot$}
\thinspace\text{ }}}
\title{Quizz 2}
\author{Romil Kadia(16105045) }
\date{April 5, 2017}

\begin{document}

\maketitle

\section{Given}
Free energy expression for Neo-Hookean material is given by:\\
\\
$\psi_{0}= \frac{\mu}{2} {(I_{1}-3)} - {\mu}lnJ + \frac{\lambda}{2} {(lnJ)^2}    $   
\section{Calculation of PK2}
The principal direction of ${\varepsilon}$ and ${\sigma}$ are same for hyper elastic material similar to isotropic material\\
\\
${S_{ij}}= \frac{\partial\psi_{0}}{\partial E_{ij}}$\\
\\
but, ${E_{ij}}= \frac{1}{2} {(C_{ij})-{\delta_{ij}}}$\\
\therefore $\partial E_{ij}= \frac{\partial C_{ij}}{2}$\\
using this in above equation\\
\therefore$S_{ij}$= $2\frac{\partial\psi_{0}}{\partial C_{ij}}$\\

$= 2[\frac{\partial \psi_{0}}{\partial I_{1}} \frac{\partial I_{1}}{\partial C_{ij}} + \frac{\partial \psi_{0}}{\partial I_{2}} \frac{\partial I_{2}}{\partial C_{ij}} + \frac{\partial \psi_{0}}{\partial I_{3}} \frac{\partial I_{3}}{\partial C_{ij}}]$\\
Now, calculating each component separately\\
$I_{1}= tr({\undertilde{C}})= \delta_{ij}C_{ij}$\\
$\frac{\partial I_{1}}{\partial C_{ij}}$ = $\delta_{ij}$\\
$\frac{\partial \psi_{0}}{\partial I_{1}}$ $\frac{\partial I_{1}}{\partial C_{ij}}$ = $\frac{\mu}{2}\frac{\partial I_{1}}{\partial C_{ij}}$\\
\\
\therefore$\frac{\partial \psi_{0}}{\partial I_{1}}$ $\frac{\partial I_{1}}{\partial C_{ij}}$=$\frac{\mu}{2} \delta_{ij}$\\
$\frac{\partial \psi_{0}}{\partial I_{2}}=0$\\
$\frac{\partial \psi_{0}}{\partial I_{3}}=\frac{\partial }{\partial I_{3}}(-\frac{\mu}{2}luI_{3} +\frac{\lambda}{2}\frac{(lnI_{3})^2}{2})$\\

=$\frac{\lambda ln(I_{3})}{cI_{3}}-\frac{\mu}{cI_{3}}$\\
And $\frac{\partial I_{3}}{\partial C_{ij}}$= $(detC_{ij}) {C_{ij}}^{-1}$\\
\\
\therefore$S_{ij}= \mu\delta_{ij}- \mu {C_{ij}}^{-1} + \lambda ln(J){C_{ij}}^{-1}$\\
\section{Cauchy Stress}
$\undertilde{\sigma}$= $J^{-1} \undertilde{F} \undertilde{S} \undertilde{F}^{T}$\\
but $\undertilde{C}=\undertilde{F}^{T}\undertilde{F}$\\
\therefore $\undertilde{S}=\mu(I-\undertilde{F}^{-1}\undertilde{F}^{-T})+\lambda lnJ (\undertilde{F}^{-1}\undertilde{F}^{-T})$\\
\therefore $\undertilde{\sigma}= \frac{\mu}{J}(\undertilde{B}-I) + (\frac{\lambda}{J} lnJ)I$\\
\section{Relating Trusdell and Jauman for Kirchoff stress}
$\undertilde{C}^{J} J^{-1} = \undertilde{C}^{T} +\undertilde{C}^{\prime}$\\
where: $\undertilde{C^\prime}:\undertilde{D} = \undertilde{D}\undertilde{\sigma} - \undertilde{\sigma}\undertilde{D}$\\
\therefore $\undertilde{C^\prime} = \frac{\partial}{\partial\undertilde{D}} (\undertilde{D}\undertilde{\sigma} -\undertilde{\sigma}\undertilde{D})$\\
$C^\prime _{ijkl} = \frac{1}{2} [\delta_{ik}\sigma_{jl} + \delta_{il}\sigma_{jk} + \delta_{jk}\sigma_{il} + \delta_{jl}\sigma_{ik}]$\\
\\
substituting the value of $\sigma$ in above equation:\\
$C^\prime _{ijkl} = \frac{\mu}{2J} (\delta_{ik}B_{jl} + \delta_{il}B_{jk} + \delta_{jk}B_{il} + \delta_{jl}B_{ik}) + \frac{\lambda lnJ - \mu}{J} (\delta_{ik}\delta_{jl} + \delta_{il}\delta_{jk})$\\
\\
Now, Trusdell stress:\\
$\hat{\sigma} = \frac{1}{J} (\undertilde{F} \undertilde{\dot{S}} \undertilde{F^T})$\\
But, $\undertilde{\dot{S}} = \undertilde{C}: D(\undertilde{E})$\\
$\hat{\sigma}= \frac{1}{J} (\undertilde{F}(\undertilde{C}:\undertilde{\dot{E}})\undertilde{F^T})$\\
\\
using the relation between E and F:\\
$\therefore  \hat{\sigma} = \frac{1}{J} (\undertilde{F}(\undertilde{C}:\undertilde{F^T} \undertilde{D} \undertilde{F})\undertilde{F^T})$\\
in indicial:
$\sigma_{ij} = \frac{1}{J} C_{mnop} F_{im}F_{qo}F_{rp}F_{jn}D_{qr}$\\
\\
Defining elastic constant for trusdell stress:\\
$C^T_{ijkl} = \frac{1}{J} C_{mnop} F_{im}F_{jn}F_{kl}F_{lp}$\\
\\
Here $C_{mnop}$ is the elastic constant for PK2 given by:\\
$\undertilde{S} = \undertilde{C}^{SE}} :\undertilde{E}$\\
$\therefore C^{SE}_{ijkl} = 2\frac{\partial S_{ij}}{\partial C_{kl}}$\\

$= \frac{\partial}{\partial C_{kl}} (\mu(\delta_{ij}-C^{-1}_{ij}) -\lambda lnJ C^{-1}_{ij})$\\

$= (\mu + \lambda lnJ)(C^{-1}_{ik}C^{-1}_{jl} + C^{-1}_{il}C^{-1}_{jk}) + \lambda C^{-1}_{ij}C^{-1}_{kl}$\\
\\
But we know that:\\
$C^{-1}_{ij} = F^{-1}_{ix} F^{-1}_{jx}$\\
\\
substituting $C^{-1} $value in $C^{SE}$ and using that in $C^{T}$\\
\therefore $C^{T}_{ijkl} = [\frac{(\mu - \lambda lnJ)}{J} (F^{-1}_{mu}F^{-1}_{oy}F^{-1}_{nv}F^{-1}_{pv} + F^{-1}_{mw}F^{-1}_{nw}F^{-1}_{ox}F^{-1}_{px}) + \frac{\lambda}{J} F^{-1}_{my}F^{-1}_{ny}F^{-1}_{oz}F^{-1}_{pz}] F_{im}F_{jn}F_{ko}F_{lp} $\\
\\
After further simplification trusdell elastic constant:\\
$C^{T}_{ijkl} = \frac{(\mu - \lambda lnJ)}{J} (\delta_{ik}\delta_{jl} + \delta_{il}\delta_{jk}) + \frac{\lambda}{J}(\delta_{ij}\delta_{kl})$\\
\\
Substituting the expression of $C\prime$ and $C^{T}$ in $C^{J}$\\
$C^{J}_{ijkl}J^{-1} = \frac{(\mu - \lambda lnJ)}{J} (\delta_{ik}\delta_{jl} + \delta_{il}\delta_{jk}) + \frac{\lambda}{J}(\delta_{ij}\delta_{kl}) + \frac{\mu}{2J} (\delta_{ik}B_{jl} + \delta_{il}B_{jk} + \delta_{jk}B_{il} + \delta_{jl}B_{ik}) + \frac{\lambda lnJ - \mu}{J} (\delta_{ik}\delta_{jl} + \delta_{il}\delta_{jk})$\\
\\
\therefore $C^{J}_{ijkl} = \frac{\lambda}{J}(\delta_{ij}\delta_{kl}) + \frac{\mu}{2} (\delta_{ik}B_{jl} + \delta_{il}B_{jk} + \delta_{jk}B_{il} + \delta_{jl}B_{ik})$\\
\\
\section{Constitutive relation for kirchoff stress in Jauman rate}
$\undertilde{\uptau}^\nabla = \undertilde{C}^{J} : \undertilde{D}$\\
\\
\section{Tangent stiffness matrix}
$\undertilde{C}=$
\begin{bmatrix}
$\lambda + 2\mu B_{11} & \lambda & \lambda & \mu B_{12} & \mu B_{13} & 0 $\\
$ -- & \lambda +2\mu B_{22} & \lambda & \mu B_{21} & 0 & \mu B_{23}$\\
$ -- & -- & \lambda + 2\mu B_{33} & 0 & \mu B_{31} & \mu B_{32}$\\
$ -- & -- & -- & \frac{\mu}{2} (B_{11} + B_{22}) & \frac{\mu}{2} B_{23} & \frac{\mu}{2} B_{13}$\\
$ -- & -- & -- & -- & \frac{\mu}{2} (B_{11} + B_{33}) & \frac{\mu}{2} B_{12}$\\
$ sym & -- & -- & -- & -- & \frac{\mu}{2} (B_{22} + B_{33})$
\end{bmatrix}

\end{document}